src/spec/TLS13.Wire.Spec.Reveal.Alert.fst
@@ -1,0 +1,50 @@
+module TLS13.Wire.Spec.Reveal.Alert
+
+friend TLS13.Wire.Spec
+
+module B = TLS13.Bytes
+module M = TLS13.Messages
+module Seq = FStar.Seq
+module T = TLS13.Types
+module U8 = FStar.UInt8
+module WS = TLS13.Wire.Spec
+
+private let lemma_nat_of_byte_reveal (b:B.byte)
+  : Lemma (WS.nat_of_byte b == U8.v b) =
+  ()
+
+private let lemma_alert_description_of_byte_reveal (b:B.byte)
+  : Lemma (WS.alert_description_of_byte b ==
+      (match U8.v b with
+       | 0   -> Some T.CloseNotify
+       | 10  -> Some T.UnexpectedMessage
+       | 20  -> Some T.BadRecordMac
+       | 40  -> Some T.HandshakeFailure
+       | 46  -> Some T.CertificateUnknown
+       | 47  -> Some T.IllegalParameter
+       | 50  -> Some T.DecodeError
+       | 51  -> Some T.DecryptError
+       | 70  -> Some T.ProtocolVersion
+       | 110 -> Some T.UnsupportedExtension
+       | _   -> None)) =
+  lemma_nat_of_byte_reveal b;
+  match WS.nat_of_byte b with
+  | 0 -> assert (U8.v b == 0)
+  | 10 -> assert (U8.v b == 10)
+  | 20 -> assert (U8.v b == 20)
+  | 40 -> assert (U8.v b == 40)
+  | 46 -> assert (U8.v b == 46)
+  | 47 -> assert (U8.v b == 47)
+  | 50 -> assert (U8.v b == 50)
+  | 51 -> assert (U8.v b == 51)
+  | 70 -> assert (U8.v b == 70)
+  | 110 -> assert (U8.v b == 110)
+  | _ -> ()
+
+let lemma_ptm_alert fragment =
+  if B.length fragment == 2 then (
+    assert (B.length fragment == 2);
+    lemma_alert_description_of_byte_reveal (Seq.index fragment 1)
+  ) else (
+    assert (not (B.length fragment == 2))
+  )
