src/spec/TLS13.Wire.Spec.Reveal.Alert.fsti
@@ -1,0 +1,28 @@
+module TLS13.Wire.Spec.Reveal.Alert
+
+module B = TLS13.Bytes
+module M = TLS13.Messages
+module Seq = FStar.Seq
+module T = TLS13.Types
+module U8 = FStar.UInt8
+module WS = TLS13.Wire.Spec
+
+val lemma_ptm_alert:
+  fragment:B.bytes ->
+  Lemma (ensures (
+    if B.length fragment == 2
+    then
+      WS.parse_tls_message T.Alert fragment ==
+        (match U8.v (Seq.index fragment 1) with
+         | 0   -> Some (M.TlsAlert T.CloseNotify)
+         | 10  -> Some (M.TlsAlert T.UnexpectedMessage)
+         | 20  -> Some (M.TlsAlert T.BadRecordMac)
+         | 40  -> Some (M.TlsAlert T.HandshakeFailure)
+         | 46  -> Some (M.TlsAlert T.CertificateUnknown)
+         | 47  -> Some (M.TlsAlert T.IllegalParameter)
+         | 50  -> Some (M.TlsAlert T.DecodeError)
+         | 51  -> Some (M.TlsAlert T.DecryptError)
+         | 70  -> Some (M.TlsAlert T.ProtocolVersion)
+         | 110 -> Some (M.TlsAlert T.UnsupportedExtension)
+         | _   -> None)
+    else WS.parse_tls_message T.Alert fragment == None))
