src/spec/TLS13.Wire.Spec.Reveal.ClientHello.Parseback.Extensions.fsti
@@ -1,0 +1,44 @@
+module TLS13.Wire.Spec.Reveal.ClientHello.Parseback.Extensions
+
+module B = TLS13.Bytes
+module Seq = FStar.Seq
+module LP = LowParse.Spec
+module GHN = TLS13.Wire.Generated.HostName
+module GSNM = TLS13.Wire.Generated.ServerName
+module GSNL = TLS13.Wire.Generated.ServerNameList
+module GSNE = TLS13.Wire.Generated.ExtensionClientHello_extension_data_server_name
+module GKSEKE = TLS13.Wire.Generated.KeyShareEntry_key_exchange
+module GNG = TLS13.Wire.Generated.NamedGroup
+module GKSE = TLS13.Wire.Generated.KeyShareEntry
+module GSS = TLS13.Wire.Generated.SignatureScheme
+module GPV = TLS13.Wire.Generated.ProtocolVersion
+module GECH = TLS13.Wire.Generated.ExtensionClientHello
+
+val lemma_lp_sg_extension ()
+  : Lemma (Seq.equal (LP.serialize GECH.extensionClientHello_serializer (GECH.Extension_data_supported_groups [GNG.X25519]))
+                     (B.of_list [0uy; 0x0auy; 0uy; 4uy; 0uy; 2uy; 0uy; 0x1duy]))
+
+val lemma_lp_sa_extension ()
+  : Lemma (Seq.equal (LP.serialize GECH.extensionClientHello_serializer
+                        (GECH.Extension_data_signature_algorithms [GSS.Rsa_pss_rsae_sha256]))
+                     (B.of_list [0uy; 0x0duy; 0uy; 4uy; 0uy; 2uy; 0x08uy; 0x04uy]))
+
+val lemma_lp_sv_extension ()
+  : Lemma (Seq.equal (LP.serialize GECH.extensionClientHello_serializer
+                        (GECH.Extension_data_supported_versions [GPV.TLS_1p3]))
+                     (B.of_list [0uy; 0x2buy; 0uy; 3uy; 2uy; 0x03uy; 0x04uy]))
+
+val lemma_lp_ks_extension (key: GKSEKE.keyShareEntry_key_exchange{Seq.length key == 32})
+  : Lemma (Seq.equal (LP.serialize GECH.extensionClientHello_serializer
+                        (GECH.Extension_data_key_share ([ { GKSE.group = GNG.X25519; GKSE.key_exchange = key } ])))
+                     (Seq.append (B.of_list [0uy; 0x33uy; 0uy; 38uy; 0uy; 36uy; 0uy; 0x1duy; 0uy; 32uy]) key))
+
+val mk_snl (hn: GHN.hostName{Seq.length hn <= 255}) : GSNL.serverNameList
+
+val mk_sne (hn: GHN.hostName{Seq.length hn <= 255})
+  : GSNE.extensionClientHello_extension_data_server_name
+
+val lemma_lp_sn_extension (hn: GHN.hostName{Seq.length hn <= 255 /\ Seq.length hn > 0})
+  : Lemma (Seq.equal (LP.serialize GECH.extensionClientHello_serializer
+                        (GECH.Extension_data_server_name (mk_sne hn)))
+                     (TLS13.Wire.Spec.Reveal.ClientHello.client_hello_server_name_extension_bytes hn))
