src/spec/TLS13.Wire.Spec.Reveal.ClientHello.Parseback.fst
@@ -1,0 +1,88 @@
+module TLS13.Wire.Spec.Reveal.ClientHello.Parseback
+friend TLS13.Wire.Generated.ProtocolVersion
+friend TLS13.Wire.Generated.Random
+friend TLS13.Wire.Generated.CipherSuite
+friend TLS13.Wire.Generated.ClientHello_legacy_session_id
+friend TLS13.Wire.Generated.ClientHello_cipher_suites
+friend TLS13.Wire.Generated.ClientHello_legacy_compression_methods
+friend TLS13.Wire.Generated.ExtensionClientHello
+friend TLS13.Wire.Generated.ClientHello_extensions
+friend TLS13.Wire.Generated.ClientHello
+friend TLS13.Wire.Spec
+
+module B = TLS13.Bytes
+module M = TLS13.Messages
+module T = TLS13.Types
+module Seq = FStar.Seq
+module WS = TLS13.Wire.Spec
+module LP = LowParse.Spec
+module RCH = TLS13.Wire.Spec.Reveal.ClientHello
+module GPV = TLS13.Wire.Generated.ProtocolVersion
+module GRandom = TLS13.Wire.Generated.Random
+module GSID = TLS13.Wire.Generated.ClientHello_legacy_session_id
+module GComp = TLS13.Wire.Generated.ClientHello_legacy_compression_methods
+module GCS = TLS13.Wire.Generated.CipherSuite
+module GCH = TLS13.Wire.Generated.ClientHello
+module PBL = TLS13.Wire.Spec.Reveal.ClientHello.Parseback.Low
+
+let client_hello_body_bytes random hostname key_share = RCH.client_hello_body_bytes random hostname key_share
+let lemma_client_hello_body_bytes_reveal hello = RCH.lemma_client_hello_body_bytes_reveal hello
+let lemma_client_hello_extensions_len hostname key_share = RCH.lemma_client_hello_extensions_len hostname key_share
+
+#push-options "--split_queries always --fuel 8 --ifuel 2 --z3rlimit 80"
+let lemma_parse_client_hello_serialize_client_hello
+  (ch:M.client_hello{ch.M.cipher_suites == [T.TLS_CHACHA20_POLY1305_SHA256] /\
+                    ch.M.signature_schemes == [T.RsaPssRsaeSha256] /\
+                    (match ch.M.server_name with
+                     | None -> True
+                     | Some hostname -> B.length hostname <= 255)})
+  : Lemma
+      (requires (match ch.M.server_name with
+                 | None -> True
+                 | Some hostname -> B.length hostname > 0))
+      (ensures WS.parse_client_hello (WS.serialize_client_hello ch) == Some ch)
+=
+  match ch.M.server_name with
+  | Some hostname ->
+    assert (B.length hostname <= 255);
+    assert (B.length hostname > 0);
+    lemma_client_hello_body_bytes_reveal ch;
+    lemma_client_hello_extensions_len hostname ch.M.key_share;
+    let low : GCH.clientHello =
+      { GCH.legacy_version = GPV.TLS_1p2;
+        GCH.random = ch.M.random;
+        GCH.legacy_session_id = B.empty;
+        GCH.cipher_suites = [GCS.TLS_CHACHA20_POLY1305_SHA256];
+        GCH.legacy_compression_methods = B.of_list [0uy];
+        GCH.extensions = PBL.mk_ext_list_some hostname ch.M.key_share } in
+    PBL.lemma_lp_ch_low_bytes_some ch hostname;
+    Seq.lemma_eq_elim
+      (LP.serialize GCH.clientHello_serializer low)
+      (client_hello_body_bytes ch.M.random hostname ch.M.key_share);
+    Seq.lemma_eq_elim
+      (WS.serialize_client_hello ch)
+      (client_hello_body_bytes ch.M.random hostname ch.M.key_share);
+    LP.parse_serialize GCH.clientHello_serializer low;
+    assert_norm (WS.synth_client_hello low == Some ch);
+    assert (WS.parse_client_hello (WS.serialize_client_hello ch) == Some ch)
+  | None ->
+    lemma_client_hello_body_bytes_reveal ch;
+    lemma_client_hello_extensions_len B.empty ch.M.key_share;
+    let low : GCH.clientHello =
+      { GCH.legacy_version = GPV.TLS_1p2;
+        GCH.random = ch.M.random;
+        GCH.legacy_session_id = B.empty;
+        GCH.cipher_suites = [GCS.TLS_CHACHA20_POLY1305_SHA256];
+        GCH.legacy_compression_methods = B.of_list [0uy];
+        GCH.extensions = PBL.mk_ext_list_none ch.M.key_share } in
+    PBL.lemma_lp_ch_low_bytes_none ch;
+    Seq.lemma_eq_elim
+      (LP.serialize GCH.clientHello_serializer low)
+      (client_hello_body_bytes ch.M.random B.empty ch.M.key_share);
+    Seq.lemma_eq_elim
+      (WS.serialize_client_hello ch)
+      (client_hello_body_bytes ch.M.random B.empty ch.M.key_share);
+    LP.parse_serialize GCH.clientHello_serializer low;
+    assert_norm (WS.synth_client_hello low == Some ch);
+    assert (WS.parse_client_hello (WS.serialize_client_hello ch) == Some ch)
+#pop-options
