src/spec/TLS13.Wire.Spec.Reveal.ClientHello.Parseback.fsti
@@ -1,0 +1,18 @@
+module TLS13.Wire.Spec.Reveal.ClientHello.Parseback
+
+module B = TLS13.Bytes
+module M = TLS13.Messages
+module T = TLS13.Types
+module WS = TLS13.Wire.Spec
+
+val lemma_parse_client_hello_serialize_client_hello
+  (ch:M.client_hello{ch.M.cipher_suites == [T.TLS_CHACHA20_POLY1305_SHA256] /\
+                     ch.M.signature_schemes == [T.RsaPssRsaeSha256] /\
+                     (match ch.M.server_name with
+                      | None -> True
+                      | Some hostname -> B.length hostname <= 255)})
+  : Lemma
+      (requires (match ch.M.server_name with
+                 | None -> True
+                 | Some hostname -> B.length hostname > 0))
+      (ensures WS.parse_client_hello (WS.serialize_client_hello ch) == Some ch)
