src/spec/TLS13.Wire.Spec.Reveal.Finished.fsti
@@ -1,0 +1,18 @@
+module TLS13.Wire.Spec.Reveal.Finished
+
+module B = TLS13.Bytes
+module M = TLS13.Messages
+module Seq = FStar.Seq
+module T = TLS13.Types
+module WS = TLS13.Wire.Spec
+
+val lemma_serialize_finished_reveal:
+  fin:M.finished ->
+  Lemma (Seq.equal
+    (WS.serialize_handshake (M.Finished fin))
+    (B.append (B.of_list [20uy; 0uy; 0uy; 32uy]) fin.M.verify_data))
+
+val lemma_parse_finished_handshake:
+  fin:M.finished ->
+  Lemma (WS.parse_tls_message T.Handshake (WS.serialize_handshake (M.Finished fin)) ==
+         Some (M.TlsHandshake (M.Finished fin)))
